feat: FromCBOR instances for basic types

KLR/Serde/Basic.lean
@@ -4,6 +4,8 @@ Released under Apache 2.0 license as described in the file LICENSE.
 Authors: Paul Govereau, Sean McLaughlin
 -/
 import KLR.Util
+import Plausible
+import TensorLib  -- for all the nice conversion functions
 
 /-
 # Encoding and Decoding of Basic CBOR values
@@ -20,16 +22,54 @@ class ToCBOR (a : Type u) where
 export ToCBOR (toCBOR)
 
 class FromCBOR (a : Type u) where
-  parseCBOR' (arr : ByteArray) : Err (Nat × a)
+  parse (arr : ByteArray) : Err (Nat × a)
 
-export FromCBOR (parseCBOR')
+open FromCBOR (parse)
 
 def parseCBOR [FromCBOR a] (arr : ByteArray) : Err (ByteArray × a) :=
-  (parseCBOR' arr).map fun (sz, x) =>
+  (parse arr).map fun (sz, x) =>
     (.mk (arr.data.drop sz), x)
 
 def fromCBOR [FromCBOR a] (arr : ByteArray) : Err a :=
-  (parseCBOR' arr).map Prod.snd
+  (parse arr).map Prod.snd
+
+
+-- Often we want to modify an encoding by adding some additional bits to the type tag
+private def adjustTag (bit : UInt8) (a : ByteArray) : ByteArray :=
+  .mk $ a.data.set! 0 (a.data[0]! ||| bit)
+
+-- Prepend a tag byte to an existing ByteAarray
+private def withTag (tag : UInt8) (arr : ByteArray) : ByteArray :=
+  let res := ByteArray.emptyWithCapacity (arr.size + 1)
+  let res := res.push tag
+  ByteArray.copySlice arr 0 res 1 arr.size (exact := true)
+
+-- Parse a value and then apply a transformation
+private def parseMap (a : Type) [FromCBOR a] (f : a -> b) (arr : ByteArray) : Err (Nat × b) := do
+  let (sz, x) <- parse arr
+  return (sz, f x)
+
+/-
+For testing with Plausible we override the Float instances
+to avoid NaN in these because they cause false negatives on
+round-trip tests.
+-/
+local instance : Plausible.SampleableExt Float32 :=
+  Plausible.SampleableExt.mkSelfContained do
+    let x <- Plausible.Gen.chooseNatLt 0 UInt32.size (Nat.zero_lt_succ _)
+    let f := Float32.ofBits x.val.toUInt32
+    return if f.isNaN then 0.0 else f
+
+local instance : Plausible.SampleableExt Float :=
+  Plausible.SampleableExt.mkSelfContained do
+    let x <- Plausible.Gen.chooseNatLt 0 UInt64.size (Nat.zero_lt_succ _)
+    let f := Float.ofBits x.val.toUInt64
+    return if f.isNaN then 0.0 else f
+
+private def roundtrip [BEq a] [ToCBOR a] [FromCBOR a] (x : a) : Bool :=
+  match fromCBOR (toCBOR x) with
+  | .error _ => false
+  | .ok y => x == y
 
 /-
 # Booleans
@@ -41,7 +81,7 @@ instance : ToCBOR Bool where
     | true  => .mk #[0xf5]
 
 instance : FromCBOR Bool where
-  parseCBOR' arr := do
+  parse arr := do
     if h:arr.size > 0 then
       match arr[0]'h with
       | 0xf4 => return (1, false)
@@ -51,69 +91,256 @@ instance : FromCBOR Bool where
 
 -- Only two cases, so no plausible for this test
 #eval do
-  match fromCBOR (toCBOR true) with
-  | .ok true => pure ()
-  | _ => throwError "CBOR Bool mismatch: true"
-  match fromCBOR (toCBOR false) with
-  | .ok false => pure ()
-  | _ => throwError "CBOR Bool mismatch: false"
+  if roundtrip true == false then
+    throwError "CBOR Bool mismatch: true"
+  if roundtrip false == false then
+    throwError "CBOR Bool mismatch: false"
 
 /-
-# Integers
+# 8-bit integers
 -/
 
 instance : ToCBOR UInt8 where
   toCBOR x :=
-    if x <= 23 then .mk #[x]
-    else .mk #[ 0x18, x ]
+    if x < 0x18 then .mk #[x]
+    else .mk #[0x18, x]
 
+instance : ToCBOR Int8 where
+  toCBOR x :=
+    if x >= 0 then toCBOR x.toUInt8
+    else adjustTag 0x20 (toCBOR (x.abs.toUInt8 - 1))
+
+/-
+This is a common pattern for the unsigned integers. If the value is less than
+our tag, then we try the next smallest integer type. Otherwise, we remove the
+tag and try to parse the value.
+-/
+private def fromFixed (arr : ByteArray) (tag : UInt8) (next f : ByteArray -> Err a) : Err a :=
+  if h:arr.size > 0 then
+    let b0 := arr[0]'h
+    if b0 < tag then
+      next arr
+    else if b0 == tag then
+      f (arr.drop 1)
+    else throw s!"expecting unsigned integer (tag {tag})"
+  else throw "expecting unsigned integer: got EOF"
+
+instance : FromCBOR UInt8 where
+  parse arr := do
+    fromFixed arr 0x18
+      fun arr => return (1, arr[0]!) -- fromFixed will have checked this is OK
+      fun arr =>
+        if h:arr.size > 0 then return (2, arr[0])
+        else throw "expecting UInt8"
+
+/-
+This is a common pattern: many encodings use unsigned integers with a different
+major code (upper three bits). To handle this, we clear the upper three bits
+(major code) and try to parse the result, and return the major code, and value.
+Note, because we ara clearing the major code, the only types which will work are
+the unsigned integer types.
+-/
+private def parseUInt (a : Type) [FromCBOR a] (arr : ByteArray) : Err (UInt8 × Nat × a) := do
+  if h:arr.size > 0 then
+    let b0 := arr[0]'h
+    let major := b0 &&& 0xe0 -- top 3 bits
+    let arr := arr.set 0 (b0 &&& 0x1f) -- clear top 3 bits
+    let (sz, x) <- @parse a _ arr  -- try to parse at type a
+    return (major, sz, x)
+  throw "expecting integer"
+
+/-
+The encoding of signed and unsigned is the same except for the major type,
+which is 1 for signed instead of 0. Parse the unsigned number, check the major
+code and flip the sign if needed.
+-/
+private def checkSign (a : Type) [FromCBOR a] (arr : ByteArray) : Err (Bool × Nat × a) := do
+  let (major, sz, x) <- parseUInt a arr
+  if major == 0x00 then
+    return (false, sz, x)
+  if major == 0x20 then
+    return (true, sz, x)
+  throw "expecting integer"
+
+instance : FromCBOR Int8 where
+  parse arr := do
+    let (signed, sz, x) <- checkSign UInt8 arr
+    if signed
+    then return (sz, (x+1).toInt8.neg)
+    else return (sz, x.toInt8)
+
+-- Test vectors from RFC
 #guard (toCBOR (0 : UInt8)).data == #[0]
 #guard (toCBOR (23 : UInt8)).data == #[23]
 #guard (toCBOR (24 : UInt8)).data == #[0x18, 24]
 #guard (toCBOR (100 : UInt8)).data == #[0x18, 0x64]
 #guard (toCBOR (255 : UInt8)).data == #[0x18, 255]
 
+#guard (toCBOR (-1 : Int8)).data == #[0x20]
+#guard (toCBOR (-10 : Int8)).data == #[0x29]
+#guard (toCBOR (-100 : Int8)).data == #[0x38, 0x63]
+#guard (toCBOR Int8.maxValue).data == #[0x18, 0x7f]
+#guard (toCBOR Int8.minValue).data == #[0x38, 0x7f]
+
+/--
+info: Unable to find a counter-example
+---
+warning: declaration uses 'sorry'
+-/
+#guard_msgs in
+  example (x : UInt8) :
+    roundtrip x == true := by plausible
+
+/--
+info: Unable to find a counter-example
+---
+warning: declaration uses 'sorry'
+-/
+#guard_msgs in
+  example (x : Int8) :
+    roundtrip x == true := by plausible
+
+/-
+# 16-bit integers
+-/
+
 instance : ToCBOR UInt16 where
   toCBOR x :=
-    if x.toNat < UInt8.size then
-      toCBOR x.toUInt8
-    else
-      .mk #[ 0x19, (x >>> 8).toUInt8, x.toUInt8 ]
+    if x.toNat < UInt8.size
+    then toCBOR x.toUInt8
+    else withTag 0x19 x.toBEByteArray
 
+instance : ToCBOR Int16 where
+  toCBOR x :=
+    if x >= 0 then toCBOR x.toUInt16
+    else adjustTag 0x20 (toCBOR (x.abs.toUInt16 - 1))
+
+instance : FromCBOR UInt16 where
+  parse arr :=
+    fromFixed arr 0x19
+      (parseMap UInt8 fun x => x.toUInt16)
+      fun arr => return (3, <- (arr.take 2).toUInt16BE)
+
+instance : FromCBOR Int16 where
+  parse arr := do
+    let (signed, sz, x) <- checkSign UInt16 arr
+    if signed
+    then return (sz, (x+1).toInt16.neg)
+    else return (sz, x.toInt16)
+
+-- Test vectors from RFC
 #guard (toCBOR (0 : UInt16)).data == #[0]
 #guard (toCBOR (255 : UInt16)).data == #[0x18, 255]
 #guard (toCBOR (256 : UInt16)).data == #[0x19, 1, 0]
 #guard (toCBOR (1000 : UInt16)).data == #[0x19, 3, 0xe8]
 
+#guard (toCBOR (-1000 : Int16)).data == #[0x39, 0x03, 0xe7]
+#guard (toCBOR Int16.maxValue).data == #[0x19, 0x7f, 0xff]
+#guard (toCBOR Int16.minValue).data == #[0x39, 0x7f, 0xff]
+
+/--
+info: Unable to find a counter-example
+---
+warning: declaration uses 'sorry'
+-/
+#guard_msgs in
+  example (x : UInt16) :
+    roundtrip x == true := by plausible
+
+/--
+info: Unable to find a counter-example
+---
+warning: declaration uses 'sorry'
+-/
+#guard_msgs in
+  example (x : Int16) :
+    roundtrip x == true := by plausible
+
+/-
+# 32-bit integers
+-/
+
 instance : ToCBOR UInt32 where
   toCBOR x :=
-    if x.toNat < UInt16.size then
-      toCBOR x.toUInt16
-    else
-      .mk #[0x1a, (x >>> 24).toUInt8,
-                  (x >>> 16).toUInt8,
-                  (x >>>  8).toUInt8,
-                  (x >>>  0).toUInt8 ]
+    if x.toNat < UInt16.size
+    then toCBOR x.toUInt16
+    else withTag 0x1a x.toBEByteArray
 
+instance : ToCBOR Int32 where
+  toCBOR x :=
+    if x >= 0 then toCBOR x.toUInt32
+    else adjustTag 0x20 (toCBOR (x.abs.toUInt32 - 1))
+
+instance : FromCBOR UInt32 where
+  parse arr :=
+    fromFixed arr 0x1a
+      (parseMap UInt16 fun x => x.toUInt32)
+      fun arr => return (5, <- (arr.take 4).toUInt32BE)
+
+instance : FromCBOR Int32 where
+  parse arr := do
+    let (signed, sz, x) <- checkSign UInt32 arr
+    if signed
+    then return (sz, (x+1).toInt32.neg)
+    else return (sz, x.toInt32)
+
+-- Test vectors from RFC
 #guard (toCBOR (0 : UInt32)).data == #[0]
 #guard (toCBOR (255 : UInt32)).data == #[0x18, 255]
 #guard (toCBOR (256 : UInt32)).data == #[0x19, 1, 0]
 #guard (toCBOR (1000000 : UInt32)).data == #[0x1a, 0, 0x0f, 0x42, 0x40]
 
+#guard (toCBOR (-1000000 : Int32)).data == #[0x3a, 0, 0x0f, 0x42, 0x3f]
+#guard (toCBOR Int32.maxValue).data == #[0x1a, 0x7f, 0xff, 0xff, 0xff]
+#guard (toCBOR Int32.minValue).data == #[0x3a, 0x7f, 0xff, 0xff, 0xff]
+
+/--
+info: Unable to find a counter-example
+---
+warning: declaration uses 'sorry'
+-/
+#guard_msgs in
+  example (x : UInt32) :
+    roundtrip x == true := by plausible
+
+/--
+info: Unable to find a counter-example
+---
+warning: declaration uses 'sorry'
+-/
+#guard_msgs in
+  example (x : Int32) :
+    roundtrip x == true := by plausible
+
+/-
+# 64-bit integers
+-/
+
 instance : ToCBOR UInt64 where
   toCBOR x :=
-    if x.toNat < UInt32.size then
-      toCBOR x.toUInt32
-    else
-      .mk #[0x1b, (x >>> 56).toUInt8,
-                  (x >>> 48).toUInt8,
-                  (x >>> 40).toUInt8,
-                  (x >>> 32).toUInt8,
-                  (x >>> 24).toUInt8,
-                  (x >>> 16).toUInt8,
-                  (x >>>  8).toUInt8,
-                  (x >>>  0).toUInt8 ]
+    if x.toNat < UInt32.size
+    then toCBOR x.toUInt32
+    else withTag 0x1b x.toBEByteArray
 
+instance : ToCBOR Int64 where
+  toCBOR x :=
+    if x >= 0 then toCBOR x.toUInt64
+    else adjustTag 0x20 (toCBOR (x.abs.toUInt64 - 1))
+
+instance : FromCBOR UInt64 where
+  parse arr :=
+    fromFixed arr 0x1b
+      (parseMap UInt16 fun x => x.toUInt64)
+      fun arr => return (9, <- (arr.take 8).toUInt64BE)
+
+instance : FromCBOR Int64 where
+  parse arr := do
+    let (signed, sz, x) <- checkSign UInt64 arr
+    if signed
+    then return (sz, (x+1).toInt64.neg)
+    else return (sz, x.toInt64)
+
+-- Test vectors from RFC
 #guard (toCBOR (0 : UInt64)).data == #[0]
 #guard (toCBOR (255 : UInt64)).data == #[0x18, 255]
 #guard (toCBOR (256 : UInt64)).data == #[0x19, 1, 0]
@@ -123,99 +350,120 @@ instance : ToCBOR UInt64 where
 #guard (toCBOR (18446744073709551615 : UInt64)).data ==
                 #[0x1b, 0xff, 0xff, 0xff, 0xff, 0xff, 0xff, 0xff, 0xff]
 
-
--- Convert a Nat to a big-endian byte array
-private def bytesOfNat (n : Nat) : Array UInt8 :=
-  let rec loop n :=
-    if n == 0 then #[]
-    else (loop (n >>> 8)).push n.toUInt8
-   termination_by n
-   decreasing_by induction n; trivial; omega
-  loop n
-
-instance : ToCBOR Nat where
-  toCBOR x :=
-    if x < UInt64.size then
-      toCBOR x.toUInt64
-    else
-      let bytes := bytesOfNat x
-      let tag := (toCBOR bytes.size.toUInt64).data
-      let tag := tag.set! 0 (tag[0]! ||| 0x40)
-      .mk (#[0xc2] ++ tag ++ bytes)
-
-#guard (toCBOR (0 : Nat)).data == #[0]
-#guard (toCBOR (1000000000000 : Nat)).data ==
-                #[0x1b, 0, 0, 0, 0xe8, 0xd4, 0xa5, 0x10, 0]
-#guard (toCBOR (18446744073709551615 : Nat)).data ==
-                #[0x1b, 0xff, 0xff, 0xff, 0xff, 0xff, 0xff, 0xff, 0xff]
-#guard (toCBOR (18446744073709551616 : Nat)).data ==
-                #[0xc2, 0x49, 1, 0, 0, 0, 0, 0, 0, 0, 0]
-
--- negative integers a similar to positive ones with an extra bit set
-private def adjustTag (bit : UInt8) (a : ByteArray) : ByteArray :=
-  .mk $ a.data.set! 0 (a.data[0]! ||| bit)
-
-instance : ToCBOR Int8 where
-  toCBOR x :=
-    if x >= 0 then toCBOR x.toUInt8
-    else adjustTag 0x20 (toCBOR (x.abs.toUInt8 - 1))
-
-#guard (toCBOR (-1 : Int8)).data == #[0x20]
-#guard (toCBOR (-10 : Int8)).data == #[0x29]
-#guard (toCBOR (-100 : Int8)).data == #[0x38, 0x63]
-#guard (toCBOR Int8.maxValue).data == #[0x18, 0x7f]
-#guard (toCBOR Int8.minValue).data == #[0x38, 0x7f]
-
-instance : ToCBOR Int16 where
-  toCBOR x :=
-    if x >= 0 then toCBOR x.toUInt16
-    else adjustTag 0x20 (toCBOR (x.abs.toUInt16 - 1))
-
-#guard (toCBOR (-1000 : Int16)).data == #[0x39, 0x03, 0xe7]
-#guard (toCBOR Int16.maxValue).data == #[0x19, 0x7f, 0xff]
-#guard (toCBOR Int16.minValue).data == #[0x39, 0x7f, 0xff]
-
-instance : ToCBOR Int32 where
-  toCBOR x :=
-    if x >= 0 then toCBOR x.toUInt32
-    else adjustTag 0x20 (toCBOR (x.abs.toUInt32 - 1))
-
-#guard (toCBOR (-1000000 : Int32)).data == #[0x3a, 0, 0x0f, 0x42, 0x3f]
-#guard (toCBOR Int32.maxValue).data == #[0x1a, 0x7f, 0xff, 0xff, 0xff]
-#guard (toCBOR Int32.minValue).data == #[0x3a, 0x7f, 0xff, 0xff, 0xff]
-
-instance : ToCBOR Int64 where
-  toCBOR x :=
-    if x >= 0 then toCBOR x.toUInt64
-    else adjustTag 0x20 (toCBOR (x.abs.toUInt64 - 1))
-
 #guard (toCBOR (-1000000 : Int64)).data == #[0x3a, 0, 0x0f, 0x42, 0x3f]
 #guard (toCBOR Int64.maxValue).data == #[0x1b, 0x7f, 0xff, 0xff, 0xff, 0xff, 0xff, 0xff, 0xff]
 #guard (toCBOR Int64.minValue).data == #[0x3b, 0x7f, 0xff, 0xff, 0xff, 0xff, 0xff, 0xff, 0xff]
 
-instance : ToCBOR Int where
-  toCBOR
-    | .ofNat n => toCBOR n
-    | .negSucc n =>
-        let tag := if n < UInt64.size then 0x20 else 0x01
-        adjustTag tag (toCBOR n)
+/--
+info: Unable to find a counter-example
+---
+warning: declaration uses 'sorry'
+-/
+#guard_msgs in
+  example (x : UInt64) :
+    roundtrip x == true := by plausible
 
-#guard (toCBOR (-1000000 : Int)).data == #[0x3a, 0, 0x0f, 0x42, 0x3f]
-#guard (toCBOR (-0x1_00000000_00000000 : Int)).data == #[0x3b, 0xff, 0xff, 0xff, 0xff, 0xff, 0xff, 0xff, 0xff]
-#guard (toCBOR (-0x1_00000000_00000001 : Int)).data == #[0xc3, 0x49, 1, 0, 0, 0, 0, 0, 0, 0, 0]
+/--
+info: Unable to find a counter-example
+---
+warning: declaration uses 'sorry'
+-/
+#guard_msgs in
+  example (x : Int64) :
+    roundtrip x == true := by plausible
 
 /-
-# Strings, Lists, Arrays
+# Big integers
+
+Note: CBOR does support big integers (major type 0xc2 and 0xc3), however we
+don't want to support this on the C-side. These instance silently truncate.
 -/
 
-instance : ToCBOR ByteArray where
-  toCBOR arr :=
-    let size := toCBOR arr.size
-    let size := adjustTag 0x40 size
-    size ++ arr
+instance : ToCBOR Nat where toCBOR x := toCBOR x.toUInt64
+instance : ToCBOR Int where toCBOR x := toCBOR x.toInt64
 
-#guard (toCBOR $ ByteArray.mk #[]).data == #[0x40]
-#guard (toCBOR $ ByteArray.mk #[1,2,3,4]).data == #[0x44,1,2,3,4]
+instance : FromCBOR Nat where parse := parseMap _ UInt64.toNat
+instance : FromCBOR Int where parse := parseMap _ Int64.toInt
+
+/-
+# Floats
+
+Note, we encode all floats as either 32- or 64-bit IEEE; we do not use 16-bit
+formats. This should be OK, it just wastes a few bytes.
+-/
+
+instance : ToCBOR Float32 where
+  toCBOR f := withTag 0xfa (f.toBits.toBEByteArray)
+
+instance : ToCBOR Float where
+  toCBOR f := withTag 0xfb (f.toBits.toBEByteArray)
+
+instance : FromCBOR Float32 where
+  parse arr := do
+    if h:arr.size > 0 then
+      let b0 := arr[0]
+      if b0 == 0xfa then
+        let bits <- (arr.sub 1 4).toUInt32BE
+        return (5, Float32.ofBits bits)
+    throw "expecting float"
+
+instance : FromCBOR Float where
+  parse arr := do
+    if h:arr.size > 0 then
+      let b0 := arr[0]
+      if b0 == 0xfa then
+        let f32 : Float32 <- fromCBOR arr
+        return (5, f32.toFloat)
+      if b0 == 0xfb then
+        let bits <- (arr.sub 1 8).toUInt64BE
+        return (9, Float.ofBits bits)
+    throw "expecting float"
+
+
+-- Test vectors from RFC
+def f32_nan : Float32 := 0.0 / 0.0
+def f32_inf : Float32 := 1.0 / 0.0
+def f32_minf : Float32 := -1.0 / 0.0
+
+#guard (toCBOR (0 : Float32)).data == #[0xfa, 0, 0, 0, 0]
+#guard (toCBOR (-0 : Float32)).data == #[0xfa, 0x80, 0, 0, 0]
+#guard (toCBOR f32_nan).data == #[0xfa, 0x7f, 0xc0, 0, 0]
+#guard (toCBOR f32_inf).data == #[0xfa, 0x7f, 0x80, 0, 0]
+#guard (toCBOR f32_minf).data == #[0xfa, 0xff, 0x80, 0, 0]
+
+def f64_nan : Float := 0.0 / 0.0
+def f64_inf : Float := 1.0 / 0.0
+def f64_minf : Float := -1.0 / 0.0
+
+#guard (toCBOR (0 : Float)).data == #[0xfb, 0,0,0,0, 0,0,0,0]
+#guard (toCBOR (-0 : Float)).data == #[0xfb, 0x80, 0,0,0, 0,0,0,0]
+#guard (toCBOR f64_nan).data == #[0xfb, 0x7f, 0xf8, 0,0, 0,0,0,0]
+#guard (toCBOR f64_inf).data == #[0xfb, 0x7f, 0xf0, 0,0, 0,0,0,0]
+#guard (toCBOR f64_minf).data == #[0xfb, 0xff, 0xf0, 0,0, 0,0,0,0]
+
+/--
+info: Unable to find a counter-example
+---
+warning: declaration uses 'sorry'
+-/
+#guard_msgs in
+  example (x : Float32) :
+    roundtrip x == true := by plausible
+
+/--
+info: Unable to find a counter-example
+---
+warning: declaration uses 'sorry'
+-/
+#guard_msgs in
+  example (x : Float) :
+    roundtrip x == true := by plausible
+
+/-
+# Strings
+
+Note: there is no support for "terminated strings;" all strings must have a size.
+-/
 
 instance : ToCBOR String where
   toCBOR s :=
@@ -223,18 +471,128 @@ instance : ToCBOR String where
     let size := adjustTag 0x60 size
     size ++ s.toUTF8
 
+instance : FromCBOR String where
+  parse arr := do
+    let (major, sz, x) <- parseUInt UInt64 arr
+    if major != 0x60 then
+      throw "expecting string"
+    let x := x.toNat
+    let arr := (arr.drop sz).take x
+    match String.fromUTF8? arr with
+    | none => throw "invalid UTF8 string"
+    | some s => return (sz + x, s)
+
+-- Test vectors from RFC
 #guard (toCBOR "").data == #[0x60]
 #guard (toCBOR "a").data == #[0x61, 0x61]
 #guard (toCBOR "IETF").data == #[0x64, 0x49, 0x45, 0x54, 0x46]
 #guard (toCBOR "· ♥ ·").data == #[0x69, 194, 183, 32, 226, 153, 165, 32, 194, 183]
 
-instance [ToCBOR a] : ToCBOR (List a) where
-  toCBOR l :=
-    let size := toCBOR l.length.toUInt64
-    let size := adjustTag 0x80 size
-    let arrays := l.foldr (fun x arr => toCBOR x ++ arr) (.mk #[])
-    size ++ arrays
+/--
+info: Unable to find a counter-example
+---
+warning: declaration uses 'sorry'
+-/
+#guard_msgs in
+  example (x : String) :
+    roundtrip x == true := by plausible
 
-#guard (toCBOR ([] : List Nat)).data == #[0x80]
-#guard (toCBOR [1,2,3]).data == #[0x83,1,2,3]
-#guard (toCBOR [[1],[2,3],[4,5]]).data == #[0x83, 0x81,1, 0x82,2,3, 0x82,4,5]
+/-
+# Pairs
+
+All sequences, are encoded as CBOR "arrays" (major type 4).
+-/
+
+instance [ToCBOR a] [ToCBOR b] : ToCBOR (a × b) where
+  toCBOR p :=
+    let arr1 := toCBOR p.fst
+    let arr2 := toCBOR p.snd
+    withTag 0x82 (arr1 ++ arr2)
+
+instance [FromCBOR a] [FromCBOR b] : FromCBOR (a × b) where
+  parse arr := do
+    if h:arr.size > 0 then
+      let b0 := arr[0]
+      if b0 != 0x82 then
+        throw "expecting pair"
+      let (sz1, x) <- @parse a _ (arr.drop 1)
+      let (sz2, y) <- @parse b _ (arr.drop (1+sz1))
+      return (1 + sz1 + sz2, (x, y))
+    throw "expecting pair"
+
+-- These tests make sure we are computing the sizes correctly
+
+/--
+info: Unable to find a counter-example
+---
+warning: declaration uses 'sorry'
+-/
+#guard_msgs in
+  example (x : (String × UInt32 × Bool × Bool)) :
+    roundtrip x == true := by plausible
+
+/--
+info: Unable to find a counter-example
+---
+warning: declaration uses 'sorry'
+-/
+#guard_msgs in
+  example (x : (Float × Float32 × Bool)) :
+    roundtrip x == true := by plausible
+
+/-
+# Lists and Arrays
+
+Lists and arrays are encoded similar to pair above.
+-/
+
+instance [ToCBOR a] : ToCBOR (Array a) where
+  toCBOR l :=
+    let size := toCBOR l.size.toUInt64
+    let arrays := l.foldr (fun x arr => toCBOR x ++ arr) (.mk #[])
+    adjustTag 0x80 size ++ arrays
+
+instance [FromCBOR a] : FromCBOR (Array a) where
+  parse arr := do
+    let (major, sz, count) <- parseUInt UInt64 arr
+    if major != 0x80 then
+      throw "expecting array"
+    let mut as := #[]
+    let mut size := sz
+    let mut b := arr.drop sz
+    for _ in [:count.toNat] do
+      let (sz, x) <- @parse a _ b
+      as := as.push x
+      size := size + sz
+      b := b.drop sz
+    return (size, as)
+
+instance [ToCBOR a] : ToCBOR (List a) where
+  toCBOR l := toCBOR l.toArray
+
+instance [FromCBOR a] : FromCBOR (List a) where
+  parse := parseMap (Array a) Array.toList
+
+private def one : UInt8 := 1
+
+#guard (toCBOR ([] : List Bool)).data == #[0x80]
+#guard (toCBOR [one,2,3]).data == #[0x83,1,2,3]
+#guard (toCBOR [[one],[2,3],[4,5]]).data == #[0x83, 0x81,1, 0x82,2,3, 0x82,4,5]
+
+/--
+info: Unable to find a counter-example
+---
+warning: declaration uses 'sorry'
+-/
+#guard_msgs in
+  example (x : List Int32) :
+    roundtrip x == true := by plausible
+
+/--
+info: Unable to find a counter-example
+---
+warning: declaration uses 'sorry'
+-/
+#guard_msgs in
+  example (x : List (Bool × List UInt8)) :
+    roundtrip x == true := by plausible
