KLR/Util.lean
@@ -8,6 +8,7 @@ import Util.Base64
 import Util.Gzip
 import Util.Hex
 import Util.Json
+import Util.Plausible
 import Util.SHA256
 
 namespace KLR
