lakefile.lean
@@ -40,7 +40,7 @@ require plausible from git
   "https://github.com/leanprover-community/plausible" @ "v4.19.0"
 
 require TensorLib from git
-  "https://github.com/leanprover/TensorLib.git" @ "v0.0.6"
+  "https://github.com/leanprover/TensorLib.git" @ "v0.0.8"
 
 -- Comment the above and uncomment this for local development
 -- require TensorLib from "../TensorLib"
